compiler/src/iInfo.ml
@@ -2,3 +2,5 @@ type t = Location.i_loc * Annotations.annotations
 let dummy = Location.i_dummy, []
 let with_location (l, _) = (l, [])
 let is_inline (_, annot) = Annotations.has_symbol "inline" annot
+let update_after_call (_, annot) =
+  Annotations.has_symbol "update_after_call" annot
